common/FlatComp.v
@@ -1,0 +1,243 @@
+Require Import Relations.
+Require Import List.
+Require Import Coqlib.
+Require Import LanguageInterface Events Globalenvs Smallstep_.
+
+Open Scope smallstep_scope.
+Delimit Scope smallstep_scope with smallstep.
+
+Section FLAT_COMP.
+  Context {liA liB S1 S2} (L1: lts liA liB S1) (L2: lts liA liB S2).
+
+  Variant flat_state := | flat_st1 (s: S1) | flat_st2 (s: S2).
+
+  Inductive flat_step: flat_state -> trace -> flat_state -> Prop :=
+  | step1 s t s':
+      Step L1 s t s' -> flat_step (flat_st1 s) t (flat_st1 s')
+  | step2 s t s':
+      Step L2 s t s' -> flat_step (flat_st2 s) t (flat_st2 s').
+
+  Inductive flat_initial_state (q: query liB): flat_state -> Prop :=
+  | initial_state1 s:
+      valid_query L1 q = true ->
+      initial_state L1 q s ->
+      flat_initial_state q (flat_st1 s)
+  | initial_state2 s:
+      valid_query L2 q = true ->
+      initial_state L2 q s ->
+      flat_initial_state q (flat_st2 s).
+
+  Inductive flat_at_external: flat_state -> query liA -> Prop :=
+  | at_external1 s q:
+      at_external L1 s q ->
+      flat_at_external (flat_st1 s) q
+  | at_external2 s q:
+      at_external L2 s q ->
+      flat_at_external (flat_st2 s) q.
+
+  Inductive flat_after_external: flat_state -> reply liA -> flat_state -> Prop :=
+  | after_external1 s r s':
+      after_external L1 s r s' ->
+      flat_after_external (flat_st1 s) r (flat_st1 s')
+  | after_external2 s r s':
+      after_external L2 s r s' ->
+      flat_after_external (flat_st2 s) r (flat_st2 s').
+
+  Inductive flat_final_state: flat_state -> reply liB -> Prop :=
+  | final_state1 s r:
+      final_state L1 s r ->
+      flat_final_state (flat_st1 s) r
+  | final_state2 s r:
+      final_state L2 s r ->
+      flat_final_state (flat_st2 s) r.
+
+  Definition flat_lts :=
+    {|
+    step ge := flat_step;
+    valid_query q := valid_query L1 q || valid_query L2 q;
+    initial_state := flat_initial_state;
+    at_external := flat_at_external;
+    after_external := flat_after_external;
+    final_state := flat_final_state;
+    globalenv := tt;
+    |}.
+
+End FLAT_COMP.
+
+Notation "L1 ⊎ L2" :=  (flat_lts L1 L2)(at level 40, left associativity): lts_scope.
+
+Require Import CategoricalComp.
+
+Section IDENTITY.
+  Context {li S} (L : lts li li S).
+
+  Inductive id_state_match: (@flat_state (@id_state li) S) -> S -> Prop :=
+  | id_state_match_intro s:
+      id_state_match (flat_st2 s) s.
+
+  Lemma identity1: 1 ⊎ L ≤ L.
+  Proof.
+    apply fsim_lts_trivial_order.
+    eexists. intros se.
+    eapply forward_simulation_step with (match_states := id_state_match);
+      intros; inv H; cbn; auto; inv H0.
+    - inv H.
+    - eexists; repeat constructor; eauto.
+    - eexists; repeat constructor; eauto.
+    - exists tt. exists q1. repeat apply conj; try constructor; auto.
+      intros.  inv H0. eexists; repeat constructor; eauto.
+    - eexists; repeat constructor; eauto.
+  Qed.
+
+  Hypothesis init_state_valid: forall q s, initial_state L q s -> valid_query L q = true.
+
+  Lemma identity2: L ≤ 1 ⊎ L.
+  Proof.
+    apply fsim_lts_trivial_order.
+    eexists. intros se.
+    eapply forward_simulation_step with (match_states := fun s1 s2 => id_state_match s2 s1);
+      intros; cbn; auto.
+    - now inv H.
+    - inv H. exists (flat_st2 s1).
+      split; constructor; auto.
+      eapply init_state_valid. eauto.
+    - inv H. eexists. split; try constructor; auto.
+    - inv H. exists tt. exists q1. repeat apply conj; try constructor; auto.
+      intros. subst. eexists; repeat constructor; eauto.
+    - inv H0. eexists; repeat constructor; eauto.
+  Qed.
+
+  Theorem flat_comp_left_identity: 1 ⊎ L ≡ L.
+  Proof.
+    split; [ exact identity1 | exact identity2 ].
+  Qed.
+
+  Inductive id_state_match': (@flat_state S (@id_state li)) -> S -> Prop :=
+  | id_state_match'_intro s:
+      id_state_match' (flat_st1 s) s.
+
+  Lemma identity3: L ⊎ 1 ≤ L.
+  Proof.
+    apply fsim_lts_trivial_order.
+    eexists. intros se.
+    eapply forward_simulation_step with (match_states := id_state_match');
+      intros; inv H; cbn; rewrite? orb_false_r; auto; inv H0.
+    - eexists; repeat constructor; eauto.
+    - inv H1. inv H.
+    - eexists; repeat constructor; eauto.
+    - exists tt. exists q1. repeat apply conj; try constructor; auto.
+      intros. inv H0. eexists; repeat constructor; eauto.
+    - eexists; repeat constructor; eauto.
+  Qed.
+
+  Lemma identity4: L ≤ L ⊎ 1.
+  Proof.
+    apply fsim_lts_trivial_order.
+    eexists. intros se.
+    eapply forward_simulation_step with (match_states := fun s1 s2 => id_state_match' s2 s1);
+      intros; cbn; auto; try inv H.
+    - now rewrite orb_false_r.
+    - eexists; repeat constructor; auto.
+      eapply init_state_valid; eauto.
+    - eexists; repeat constructor; auto.
+    - exists tt. exists q1. repeat apply conj; try constructor; auto.
+      intros. subst. eexists; repeat constructor; auto.
+    - inv H0. eexists; repeat constructor; auto.
+  Qed.
+
+  Theorem flat_comp_right_identity: L ⊎ 1 ≡ L.
+  Proof.
+    split; [ exact identity3 | exact identity4 ].
+  Qed.
+
+End IDENTITY.
+
+Section DIST.
+  Context {liA liB liC S1 S2 S}
+          (L1: lts liB liC S1) (L2: lts liB liC S2)
+          (L: lts liA liB S).
+
+  Inductive dist_match_state:
+    (@comp_state (@flat_state S1 S2) S) ->
+    (@flat_state (@comp_state S1 S) (@comp_state S2 S)) -> Prop :=
+  | dist_match_state1 s1:
+      dist_match_state (st1 (flat_st1 s1)) (flat_st1 (st1 s1))
+  | dist_match_state2 s2:
+      dist_match_state (st1 (flat_st2 s2)) (flat_st2 (st1 s2))
+  | dist_match_state3 s1 s:
+      dist_match_state (st2 (flat_st1 s1) s) (flat_st1 (st2 s1 s))
+  | dist_match_state4 s2 s:
+      dist_match_state (st2 (flat_st2 s2) s) (flat_st2 (st2 s2 s)).
+
+  Lemma distributivity1: (L1 ⊎ L2) ∘ L ≤ (L1 ∘ L) ⊎ (L2 ∘ L).
+  Proof.
+    apply fsim_lts_trivial_order. eexists. intros se.
+    eapply forward_simulation_step with (match_states := dist_match_state).
+    - intros. inv H. cbn.
+      do 2 rewrite <- orb_assoc. f_equal.
+      rewrite orb_comm. rewrite <- orb_assoc. f_equal.
+      apply orb_diag.
+    - intros. inv H; inv H0; inv H.
+      + eexists; split; repeat constructor; auto.
+        cbn. now rewrite H0.
+      + eexists; split. apply initial_state2.
+        cbn. now rewrite H0. constructor; eauto.
+        constructor.
+    - intros. inv H; inv H0; inv H1; eexists; repeat constructor; auto.
+    - intros. inv H; inv H0.
+      + exists tt. eexists. repeat apply conj; repeat constructor; auto.
+        intros. inv H. inv H0. eexists; repeat constructor; auto.
+      + exists tt. eexists. repeat apply conj; repeat constructor; auto.
+        intros. inv H. inv H0. eexists; repeat constructor; auto.
+    - intros. inv H0; inv H; try inv H1.
+      + eexists; repeat constructor; auto.
+      + eexists. split; [ | constructor ]. repeat econstructor; eauto.
+      + eexists. split; [ | constructor ]. repeat econstructor; eauto.
+      + eexists. split; [ | constructor ]. repeat econstructor; eauto.
+      + eexists. split; [ | constructor ]. repeat econstructor; eauto.
+      + inv H5. eexists. split; [ | constructor ]. repeat econstructor; eauto.
+      + eexists. split; [ | constructor ]. repeat econstructor; eauto.
+      + inv H5. eexists. split; [ | constructor ]. repeat econstructor; eauto.
+  Qed.
+
+  Hypothesis init_state_valid1: forall q s, initial_state L1 q s -> valid_query L1 q = true.
+  Hypothesis init_state_valid2: forall q s, initial_state L2 q s -> valid_query L2 q = true.
+
+  Lemma distributivity2: (L1 ∘ L) ⊎ (L2 ∘ L) ≤ (L1 ⊎ L2) ∘ L.
+  Proof.
+    apply fsim_lts_trivial_order. eexists. intros se.
+    eapply forward_simulation_step with (match_states := fun s1 s2 => dist_match_state s2 s1).
+    - intros. inv H. cbn.
+      do 2 rewrite <- orb_assoc. f_equal.
+      rewrite orb_comm. rewrite orb_assoc. f_equal.
+      symmetry. apply orb_diag.
+    - intros. inv H; inv H0; inv H1.
+      + eexists. split; [ | constructor ]. repeat econstructor; eauto.
+      + eexists. split; [ | constructor ]. repeat econstructor; eauto.
+    - intros. inv H; inv H0; inv H1.
+      + eexists. split; [ | constructor ]. repeat econstructor; eauto.
+      + eexists. split; [ | constructor ]. repeat econstructor; eauto.
+    - intros. inv H; inv H0; inv H1.
+      + exists tt. exists q1. repeat apply conj; repeat constructor; auto.
+        intros. inv H. inv H0. inv H1.
+        eexists. split; [ | constructor ]. repeat econstructor; eauto.
+      + exists tt. exists q1. repeat apply conj; repeat constructor; auto.
+        intros. inv H. inv H0. inv H1.
+        eexists. split; [ | constructor ]. repeat econstructor; eauto.
+    - intros. inv H0; inv H; inv H1.
+      + eexists. split; [ | constructor ]. repeat econstructor; eauto.
+      + eexists. split; [ | constructor ]. repeat econstructor; eauto.
+      + eexists. split; [ | constructor ]. repeat econstructor; eauto.
+      + eexists. split; [ | constructor ]. repeat econstructor; eauto.
+      + eexists. split; [ | constructor ]. repeat econstructor; eauto.
+      + eexists. split; [ | constructor ]. repeat econstructor; eauto.
+      + eexists. split; [ | constructor ]. repeat econstructor; eauto.
+      + eexists. split; [ | constructor ]. repeat econstructor; eauto.
+  Qed.
+
+  Theorem flat_categorical_comp_distributivity:
+    (L1 ⊎ L2) ∘ L ≡ (L1 ∘ L) ⊎ (L2 ∘ L).
+  Proof.
+    split; [ exact distributivity1 | exact distributivity2 ].
+  Qed.
+End DIST.
